\documentclass{article}
%break lines of a long single word automatically
\usepackage{seqsplit}
\usepackage{graphicx}
\usepackage{amsmath}
\graphicspath{{Figures/}}
%set document font to Times New Roman
%\usepackage{times}
\begin{document}
\title{}
\author{}
\date{}
\maketitle

$$ h_\theta(x) = \theta_0 + \theta_1x $$
$$ J(\theta)=\frac{1}{2m}\sum_{i=1}^{m}(h_\theta(x^{(i)})-y^{(i)})^2 $$
$$ J(\theta_0, \theta_1) $$
$$ \theta_j = \theta_j-\alpha\frac{\partial J(\theta)}{\partial \theta_j}$$
Repeat until converge \{ $$tmp0: \theta_0=\theta_0-\alpha\frac{\partial J(\theta)}{\partial \theta_0}$$
$$tmp1: \theta_1=\theta_1-\alpha\frac{\partial J(\theta)}{\partial \theta_1}$$
\}

$$\frac{\partial J(\theta)}{\partial \theta_j} = \frac{\partial}{\partial \theta_j}(\frac{1}{2m}\sum_{i=1}^{m}(h_\theta(x^{(i)})-y^{(i)})^2)
=\frac{\partial}{\partial \theta_j}(\frac{1}{2m}\sum_{i=1}^{m}(\theta_0 + \theta_1x^{(i)}-y^{(i)})^2)$$
j = 0:$$\frac{\partial J(\theta)}{\partial \theta_0} = \frac{1}{m}\sum_{i=1}^{m}(h_\theta(x^{(i)})-y^{(i)})$$
j = 1:$$\frac{\partial J(\theta)}{\partial \theta_1} = \frac{1}{m}\sum_{i=1}^{m}(h_\theta(x^{(i)})-y^{(i)})\cdot x^{(i)}$$

$$h_\theta(x) = \theta_0x_0 + \theta_1x_1 + \theta_2x_2\dots + \theta_nx_n$$

Repeat until converge \{ $$\theta_j=\theta_j-\alpha\frac{\partial J(\theta)}{\partial \theta_j}=
\theta_j-\alpha\frac{1}{m}\sum_{i=1}^{m}(h_\theta(x^{(i)})-y^{(i)})\cdot x_j^{(i)}$$
\}

$$g(z)=\frac{1}{1+e^{-z}}$$
$$h_\theta(x)=g((\theta^Tx))=\frac{1}{1+e^(-\theta^Tx)}, \theta^Tx=\theta_0+\theta_1x_1+\theta_2x2+ \dots +\theta_nx_n$$

$$I_{x0}=-\log(p(x_0))$$
$$H(x)=-\sum_{i=1}^{n}p(x_i)\log(p(x_i))$$

$$D_{K||L}(p||q)=\sum_{i=1}^{n}p(x_i)\log(\frac{p(x_i)}{q(x_i)})=\sum_{i=1}^{n}p(x_i)\log(p(x_i))-\sum_{i=1}^{n}p(x_i)\log(q(x_i))$$

$$D_{K||L}(p||q)=-H+[-\sum_{i=1}^{n}p(x_i)\log(q(x_i))]$$

$$H(p,q)=-\sum_{i=1}^{n}p(x_i)\log(q(x_i))$$

$$J(\theta)=-\frac{1}{m}[\sum_{i=1}^{m}y^{(i)}\log(h_\theta(x^{(i)}))+(1-y^{(i)})\log(1-(h_\theta(x^{(i)})))]$$

Repeat until converge \{
$$\theta_j=\theta_j-\alpha\sum_{i=1}^{m}(h_\theta(x^{(i)})-y^{(i)})\cdot x_j^{(i)}$$
\}

\end{document}